Makefile
@@ -15,6 +15,7 @@ ABS_ROOT_DIR:=$(shell cygpath -m '$(ABS_ROOT_DIR)' 2>/dev/null || echo '$(ABS_RO
 
 BEDROCK2_DIR ?= $(ABS_ROOT_DIR)/bedrock2/
 export BEDROCK2_DIR
+SORTING_DIR ?= $(ABS_ROOT_DIR)/coq-stdlib-edits/
 
 bedrock2_noex:
 	$(MAKE) -C $(BEDROCK2_DIR) bedrock2_noex
@@ -25,7 +26,13 @@ clean_bedrock2:
 install_bedrock2_noex:
 	$(MAKE) -C $(BEDROCK2_DIR) install_bedrock2_noex
 
-fiat2: bedrock2_noex
+sorting:
+	$(MAKE) -C $(SORTING_DIR)
+
+clean_sorting:
+	$(MAKE) -C $(SORTING_DIR) clean
+
+fiat2: bedrock2_noex sorting
 	$(MAKE) -C $(ABS_ROOT_DIR)/fiat2
 
 clean_fiat2:
@@ -38,7 +45,7 @@ all: bedrock2_noex fiat2
 
 clean: clean_fiat2
 
-clean_deps: clean_bedrock2
+clean_deps: clean_bedrock2 clean_sorting
 
 clean_all: clean_deps clean
 
